WIP: expression parsing
Co-authored-by: Ben Manley <bdmanley@umich.edu>

Source/Dafny/AST/VMTPrinter.cs
@@ -23,18 +23,27 @@ namespace Microsoft.Dafny {
     private string STATE_MACHINE_RELATION_PREFIX = "Relation";
     private string STATE_MACHINE_ACTION_PREFIX = "Action";
 
-    public Dictionary<System.Type, Func<Expression, string>> AstDict = new Dictionary<System.Type, Func<Expression, string>>();
-
     public Dictionary<string, int> Instances;
     public HashSet<int> TypeLengthSet = new HashSet<int> { 0, 1 };
 
+    //public Expression InitExpression;
+
+    public Predicate InitPredicate;
+    public Predicate NextPredicate;
+
+    public string PrevName = null;
+
+    public string NextName = null;
+
+    // maps name of relation to names of datatypes
     public Dictionary<string, List<string>> RelationDatatypeParams = new Dictionary<string, List<string>>();
+
+    public List<Predicate> ActionPredicates = new List<Predicate>();
 
     public VMTPrinter(TextWriter wr,
                       Dictionary<string, int> datatypeInstanceCounts,
                       DafnyOptions.PrintModes printMode = DafnyOptions.PrintModes.Everything)
         : base(wr, printMode) {
-      AstDict[typeof(BinaryExpr)] = InstantiateBinaryExpr;
       Instances = datatypeInstanceCounts;
     }
 
@@ -46,22 +55,29 @@ namespace Microsoft.Dafny {
 
       ParseDatatypes(prog);
       ParsePredicates(prog);
+      BuildRelations();
+      BuildInit();
+      // BuildActions();
+      // DeclareActions();
+      // BuildNext();
     }
 
     public void ParseDatatypes(Program prog) {  // TODO TODO TODO PARSE CONSTRUCTOR(S)
-      //Console.WriteLine("DATATYPES");
       wr.WriteLine("\n; Define and enumerate transition system parameters");
+
+      int numFoundFinitizedDatatypes = 0;
 
       foreach (TopLevelDecl d in prog.DefaultModuleDef.TopLevelDecls) {
         if (d is DatatypeDecl) {
-          //Console.WriteLine("DATATYPE");
           var dd = (DatatypeDecl)d;
           var name = dd.Name;
 
           if (name == STATE_MACHINE_DATATYPE_NAME) {
             // Dealing with outer state machine datatype
+            continue;
           } else if (Instances.ContainsKey(name)) {
             // Dealing with one of our finitized datatypes
+            ++numFoundFinitizedDatatypes;
 
             var l = Convert.ToInt32(Math.Log2(Instances[name]));
             while (TypeLengthSet.Contains(l)) {
@@ -75,19 +91,36 @@ namespace Microsoft.Dafny {
               typeCheckString += "(= " + name + " " + name + i + ") ";
             }
             wr.WriteLine("(define-fun is_" + name + " ((" + name + " " + name + "_type)) Bool (or " + typeCheckString + "))");
+
+            // ParseDatatypeCtors(dd);
           } else {
-            Debug.Assert(false, "Finitized datatype '" + name + "' provided on command line but not found in Dafny program");
+            Debug.Assert(false, "Datatype '" + name + "' found in Dafny program but no finitization provided on command line.");
           }
-          // PrintDatatype(dd, 0, Path.GetFullPath(prog.FullName));
         }
       }
 
-      //Console.WriteLine("END DATATYPES");
+      Debug.Assert(numFoundFinitizedDatatypes == Instances.Count, "Command line contains finitized datatype(s) not found in Dafny program.");
     }
 
-    public void ParsePredicates(Program prog) {
-      //Console.WriteLine("PREDICATES");
+    // public void ParseDatatypeCtors(DatatypeDecl dd) {
+    //   Debug.Assert(dd.Ctors.Count == 1, "Datatype '" + dd.Name + "' has more than one constructor. This is not currently handled.");
 
+    //   DatatypeCtor ctor = dd.Ctors[0];
+
+    //   var datatypeParams = new List<string>();
+    //   foreach (Formal f in pred.Formals) {
+    //     string typeName = f.Type.ToString();
+    //     if (typeName != STATE_MACHINE_DATATYPE_NAME && !Instances.Keys.Contains(typeName)) {
+    //       Debug.Assert(false, "Relation '" + name + "' passed parameter of type '" + typeName + "' not in state machine datatypes");
+    //     }
+    //     if (typeName != STATE_MACHINE_DATATYPE_NAME) {
+    //       datatypeParams.Add(typeName);
+    //     }
+    //   }
+    //   RelationDatatypeParams.Add(name, datatypeParams);
+    // }
+
+    public void ParsePredicates(Program prog) {
       foreach (TopLevelDecl d in prog.DefaultModuleDef.TopLevelDecls) {
         if (d is ClassDecl) {
           ClassDecl cl = (ClassDecl)d;
@@ -95,17 +128,57 @@ namespace Microsoft.Dafny {
             if (mem is Function) {
               Function f = (Function)mem;
               if (f is Predicate) {
-                //Console.WriteLine("PREDICATE");
-
                 ParsePredicate((Predicate)f);
-
-                // PrintFunction(f, 0, false);
               }
             }
           }
         }
       }
+    }
 
+    public void ParsePredicate(Predicate pred) {
+      var name = pred.Name;
+
+      if (name == STATE_MACHINE_INIT_PRED_NAME) {
+        // Dealing with Init
+        Debug.Assert(pred.Formals.Count == 1 && pred.Formals[0].Type.ToString() == STATE_MACHINE_DATATYPE_NAME,
+                     "Init predicate must take exactly one parameter, of type " + STATE_MACHINE_DATATYPE_NAME);
+        InitPredicate = pred;
+      } else if (name == STATE_MACHINE_NEXT_PRED_NAME) {
+        // Dealing with Next
+        Debug.Assert(pred.Formals.Count == 2
+                     && pred.Formals[0].Type.ToString() == STATE_MACHINE_DATATYPE_NAME
+                     && pred.Formals[1].Type.ToString() == STATE_MACHINE_DATATYPE_NAME,
+                     "Next predicate must take exactly two parameters, of type " + STATE_MACHINE_DATATYPE_NAME
+                     + ". The first represents the current/previous state, the second represents the next state.");
+        NextPredicate = pred;
+      } else if (name.StartsWith(STATE_MACHINE_RELATION_PREFIX) && name != STATE_MACHINE_RELATION_PREFIX) {
+        // Dealing with a relation
+        var datatypeParams = new List<string>();
+        foreach (Formal f in pred.Formals) {
+          string typeName = f.Type.ToString();
+          if (typeName != STATE_MACHINE_DATATYPE_NAME && !Instances.Keys.Contains(typeName)) {
+            Debug.Assert(false, "Relation '" + name + "' passed parameter of type '" + typeName + "' not in state machine datatypes");
+          }
+          if (typeName != STATE_MACHINE_DATATYPE_NAME) {
+            datatypeParams.Add(typeName);
+          }
+        }
+        RelationDatatypeParams.Add(name, datatypeParams);
+      } else if (name.StartsWith(STATE_MACHINE_ACTION_PREFIX) && name != STATE_MACHINE_ACTION_PREFIX) {
+        // Dealing with an action
+        Debug.Assert(pred.Formals.Count == 2
+                     && pred.Formals[0].Type.ToString() == STATE_MACHINE_DATATYPE_NAME
+                     && pred.Formals[1].Type.ToString() == STATE_MACHINE_DATATYPE_NAME,
+                     "Action predicates must take exactly two parameters, of type " + STATE_MACHINE_DATATYPE_NAME
+                     + ". The first represents the current/previous state, the second represents the next state.");
+        ActionPredicates.Add(pred);
+      } else {
+        Debug.Assert(false, "Predicate '" + name + "' is not an action, relation, or keyword");
+      }
+    }
+
+    public void BuildRelations() {
       wr.WriteLine("\n; Declare transition system states");
       foreach (var (relation, datatypeParams) in RelationDatatypeParams) {
         var numDatatypes = datatypeParams.Count;
@@ -134,118 +207,286 @@ namespace Microsoft.Dafny {
           // if ret != 'bool_type':
           //   lemmas.append('(is_%s %s)' % (x.sort, name))
         }
-      }
-      else {
+      } else {
         for (int intraLevelIter = 0; intraLevelIter < datatypeAmounts[currIndex]; ++intraLevelIter) {
           GenRelationCombos(numDatatypes, datatypeAmounts, str + "_" + intraLevelIter, currIndex + 1);
         }
       }
     }
 
-    public void ParsePredicate(Predicate pred) {
-      var name = pred.Name;
-
-      if (name == STATE_MACHINE_INIT_PRED_NAME) {
-        // Dealing with Init
-      } else if (name == STATE_MACHINE_NEXT_PRED_NAME) {
-        // Dealing with Next
-      } else if (name.StartsWith(STATE_MACHINE_RELATION_PREFIX) && name != STATE_MACHINE_RELATION_PREFIX) {
-        // Dealing with a relation
-        var datatypeParams = new List<string>();
-        foreach (Formal f in pred.Formals) {
-          string typeName = f.Type.ToString();
-          if (typeName != STATE_MACHINE_DATATYPE_NAME && !Instances.Keys.Contains(typeName)) {
-            Debug.Assert(false, "Relation '" + name + "' passed parameter of type '" + typeName + "' not in state machine datatypes");
-          }
-          if (typeName != STATE_MACHINE_DATATYPE_NAME) {
-            datatypeParams.Add(typeName);
-          }
-        }
-        RelationDatatypeParams.Add(name, datatypeParams);
-      } else if (name.StartsWith(STATE_MACHINE_ACTION_PREFIX) && name != STATE_MACHINE_ACTION_PREFIX) {
-        // Dealing with an action
-      } else {
-        Debug.Assert(false, "Predicate '" + name + "' is not an action, relation, or keyword");
-      }
+    public void BuildInit() {
+      //base.PrintExpression(InitExpression, false);
+      PrevName = InitPredicate.Formals[0].Name;
+      NextName = null;
+      wr.Write("(define-fun .init () Bool (! ");
+      wr.Write(InstantiateExpr(InitPredicate.Body));
+      wr.Write(" :init true))\n");
+      PrevName = null;
+      NextName = null;
     }
 
-    public string InstantiateBinaryExpr(Expression e) {
+    public void BuildActions() {
+      //base.PrintExpression(InitExpression, false);
+      foreach (Predicate pred in ActionPredicates) {
+        PrevName = pred.Formals[0].Name;
+        NextName = pred.Formals[1].Name;
+        // TODO NOT DONE NOT DONE NOT DONE
+        wr.Write("(define-fun .init () Bool (! ");
+        wr.Write(InstantiateExpr(pred.Body));
+        wr.Write(" :init true))\n");
+      }
+      PrevName = null;
+      NextName = null;
+    }
+
+    public void BuildNext() {
+      //base.PrintExpression(InitExpression, false);
+      PrevName = NextPredicate.Formals[0].Name;
+      NextName = NextPredicate.Formals[1].Name;
+      // TODO NOT DONE NOT DONE NOT DONE
+      wr.Write("(define-fun .trans NOT DONE NOT DONE NOT DONE () Bool (! ");
+      wr.Write(InstantiateExpr(NextPredicate.Body));
+      wr.Write(" :init true))\n");
+      PrevName = null;
+      NextName = null;
+    }
+
+    public string InstantiateExpr(Expression e, Dictionary<string, string> replace = null) {
+      if (e is BinaryExpr) {
+        return InstantiateBinaryExpr(e, replace);
+      } else if (e is UnaryExpr) {
+        return InstantiateUnary(e, replace);
+      } else if (e is ForallExpr) {
+        return InstantiateForall(e, replace);
+      } else if (e is LiteralExpr) {
+        return InstantiateLiteral(e, replace);
+      } else if (e is ParensExpression) {
+        return InstantiateExpr(Expression.StripParens(e), replace);
+      } else if (e is FunctionCallExpr) {
+        return InstantiateFunctionCallExpr(e, replace);
+      } else if (e is ExprDotName) {
+        return InstantiateExprDotNameExpr(e, replace);
+      } else if (e is ApplySuffix) {
+        return InstantiateApplySuffixExpr(e, replace);
+      } else {
+        return UnhandledCase(e, replace);
+      }
+
+    }
+    public string InstantiateBinaryExpr(Expression e, Dictionary<string, string> replace = null) {
       //assert(e is BinaryExpr);
       Debug.Assert(e is BinaryExpr);
       var exp = (BinaryExpr)e;
       switch (exp.Op) {
         case BinaryExpr.Opcode.And:
-          return InstantiateAnd(e);
+          return InstantiateAnd(e, replace);
         case BinaryExpr.Opcode.Or:
-          return InstantiateOr(e);
-        case BinaryExpr.Opcode.Iff:
-          return InstantiateImplies(e);
+          return InstantiateOr(e, replace);
+        case BinaryExpr.Opcode.Imp:
+          return InstantiateImplies(e, replace);
         case BinaryExpr.Opcode.Eq:
-          return InstantiateEqual(e);
+          return InstantiateEqual(e, replace);
         case BinaryExpr.Opcode.Neq:
-          return InstantiateNotEqual(e);
+          return InstantiateNotEqual(e, replace);
+        case BinaryExpr.Opcode.In:
+          return InstantiateInExpr(e, replace);
         default:
-          Console.WriteLine("unsupported binary expression: " + exp.Op);
-          break;
+          return UnhandledCase(e, replace);
       }
+    }
+
+    public string InstantiateForall(Expression e, Dictionary<string, string> replace = null) {
+      Debug.Assert(e is ForallExpr);
+      string retval = "";
+      var exp = (ForallExpr)e;
+      Expression body = exp.LogicalBody();
+
+      if (replace == null) {
+        replace = new Dictionary<string, string>();
+      }
+
+      // TODO: calculate this dictionary
+      // have bound vars
+      // have 
+      List<Dictionary<string, string>> allcombs = new List<Dictionary<string, string>>();
+      Dictionary<string, string> start = new Dictionary<string, string>();
+      GenerateFinitizationHelper(ref allcombs, ref start, exp.BoundVars);
+      // TODO: figure out what allcombs is bad
+
+      // need to check variables, if of type datatype, then instantiate every instance in implies
+
+      retval += "(and ";
+      // take body of expression and instantiate for all bounded variables
+      for (int i = 0; i < allcombs.Count; ++i) {
+        foreach (var (key, val) in allcombs[i]) {
+          replace.Add(key, val);
+          wr.Write("key=" + key + " val=" + val + "\n");
+        }
+        retval += InstantiateExpr(body, replace);
+
+        foreach (var (key, val) in allcombs[i]) {
+          replace.Remove(key);
+        }
+      }
+
+      retval += ")";
+      return retval;
+    }
+
+    private void GenerateFinitizationHelper(ref List<Dictionary<string, string>> final, ref Dictionary<string, string> current, List<BoundVar> vars) {
+      if (current.Count == vars.Count) {
+        wr.Write("ADDING COMB: ");
+        foreach (var (key, val) in current) {
+          wr.Write(key + " " + val);
+        }
+        final.Add(current);
+        return;
+      }
+      int size = current.Count;
+      BoundVar v = vars[size];
+      wr.Write("boundval name=" + v.Name + " type=" + v.Type.ToString() + "\n");
+      for (int i = 0; i < Instances[v.Type.ToString()]; ++i) {
+        current.Add(v.Name, v.Type.ToString() + i);
+        GenerateFinitizationHelper(ref final, ref current, vars);
+        current.Remove(v.Name);
+      }
+    }
+
+    public string InstantiateUnary(Expression e, Dictionary<string, string> replace = null) {
+      return "UNARY";
+    }
+
+    public string InstantiateLiteral(Expression e, Dictionary<string, string> replace = null) {
+      return "LITERAL";
+    }
+
+
+    public string UnhandledCase(Expression e, Dictionary<string, string> replace = null) {
+      base.PrintExpression(e, false);
+      FunctionCallExpr exp = (FunctionCallExpr)e;
+      Debug.Assert(false, "unhandled expression");
       return "";
     }
 
-    public string InstantiateAnd(Expression e) {
+    public string InstantiateAnd(Expression e, Dictionary<string, string> replace = null) {
       BinaryExpr exp = (BinaryExpr)e;
       Debug.Assert(exp.Op == BinaryExpr.Opcode.And);
       string retval = "(ite (and ";
       retval += "(= ";
-      retval += AstDict[typeof(Expression)](exp.E0);
+      retval += InstantiateExpr(exp.E0, replace);
       retval += " bv_true) (= ";
-      retval += AstDict[typeof(Expression)](exp.E1);
+      retval += InstantiateExpr(exp.E1, replace);
       retval += " bv_true)) bv_true bv_false)";
       return retval;
     }
 
-    public string InstantiateOr(Expression e) {
+    public string InstantiateOr(Expression e, Dictionary<string, string> replace = null) {
       BinaryExpr exp = (BinaryExpr)e;
       Debug.Assert(exp.Op == BinaryExpr.Opcode.And);
       string retval = "(ite (or (= ";
-      retval += AstDict[typeof(Expression)](exp.E0);
+      retval += InstantiateExpr(exp.E0, replace);
       retval += " bv_true) (= ";
-      retval += AstDict[typeof(Expression)](exp.E1);
+      retval += InstantiateExpr(exp.E1, replace);
       retval += " bv_true)) bv_true bv_false)";
       return retval;
     }
 
-    public string InstantiateImplies(Expression e) {
+    public string InstantiateImplies(Expression e, Dictionary<string, string> replace = null) {
       BinaryExpr exp = (BinaryExpr)e;
-      Debug.Assert(exp.Op == BinaryExpr.Opcode.Iff);
+      Debug.Assert(exp.Op == BinaryExpr.Opcode.Imp);
       string retval = "(ite (=> (= ";
-      retval += AstDict[typeof(Expression)](exp.E0);
+      retval += InstantiateExpr(exp.E0, replace);
       retval += " bv_true) (= ";
-      retval += AstDict[typeof(Expression)](exp.E1);
+      retval += InstantiateExpr(exp.E1, replace);
       retval += " bv_true)) bv_true bv_false)";
       return retval;
     }
 
-    public string InstantiateEqual(Expression e) {
+    public string InstantiateEqual(Expression e, Dictionary<string, string> replace = null) {
       BinaryExpr exp = (BinaryExpr)e;
       Debug.Assert(exp.Op == BinaryExpr.Opcode.Eq);
       string retval = "(ite (= ";
-      retval += AstDict[typeof(Expression)](exp.E0);
+      retval += InstantiateExpr(exp.E0, replace);
       retval += " ";
-      retval += AstDict[typeof(Expression)](exp.E1);
+      retval += InstantiateExpr(exp.E1, replace);
       retval += ") bv_true bv_false)";
       return retval;
     }
 
-    public string InstantiateNotEqual(Expression e) {
+    public string InstantiateNotEqual(Expression e, Dictionary<string, string> replace = null) {
       BinaryExpr exp = (BinaryExpr)e;
       Debug.Assert(exp.Op == BinaryExpr.Opcode.Neq);
       string retval = "(ite (= ";
-      retval += AstDict[typeof(Expression)](exp.E0);
+      retval += InstantiateExpr(exp.E0, replace);
       retval += " ";
-      retval += AstDict[typeof(Expression)](exp.E1);
+      retval += InstantiateExpr(exp.E1, replace);
       retval += ") bv_false bv_true)";
       return retval;
     }
+
+    public string InstantiateFunctionCallExpr(Expression e, Dictionary<string, string> replace = null) {
+      FunctionCallExpr exp = (FunctionCallExpr)e;
+      string name = exp.Name;
+      string retval = "";
+      if (name.StartsWith(STATE_MACHINE_RELATION_PREFIX)) {
+        if (replace != null) {
+          List<Expression> args = exp.Args;
+          for (int i = 1; i < args.Count; ++i) {
+            NameSegment current = (NameSegment)args[i];
+            retval += "_" + replace[current.Name];
+          }
+          NameSegment first = (NameSegment)args[0];
+          if (first.Name == NextName) {
+            retval += "_next";
+          } else if (first.Name != PrevName) {
+            Debug.Assert(false, "invalid name for state machine:" + first.Name);
+          }
+        } else {
+          // is this possible?
+          Debug.Assert(false, "goofball! the impossible happened!");
+        }
+      }
+
+      return retval;
+    }
+
+    public string InstantiateApplySuffixExpr(Expression e, Dictionary<string, string> replace = null) {
+      // don't know the difference between function call expr and apply suffix expression...
+      ApplySuffix exp = (ApplySuffix)e;
+      string name = ((NameSegment)exp.Lhs).Name;
+      string retval = "";
+      if (name.StartsWith(STATE_MACHINE_RELATION_PREFIX)) {
+        if (replace != null) {
+          List<Expression> args = exp.Args;
+          for (int i = 1; i < args.Count; ++i) {
+            NameSegment current = (NameSegment)args[i];
+            retval += "_" + replace[current.Name];
+          }
+          NameSegment first = (NameSegment)args[0];
+          if (first.Name == NextName) {
+            retval += "_next";
+          } else if (first.Name != PrevName) {
+            Debug.Assert(false, "invalid name for state machine:" + first.Name);
+          }
+        } else {
+          // is this possible?
+          Debug.Assert(false, "goofball! the impossible happened!");
+        }
+      }
+
+      return retval;
+
+    }
+
+    public string InstantiateInExpr(Expression e, Dictionary<string, string> replace = null) {
+      return "IN EXPR";
+    }
+
+    public string InstantiateExprDotNameExpr(Expression e, Dictionary<string, string> replace = null) {
+      return "EXPR.NAME";
+    }
+
+
   }
 
 }
