Test/591tests/lock_server.dfy
@@ -1,11 +1,7 @@
-// type client
-// type server
 datatype Server = Server(id:int, semaphore:bool)
 datatype Client = Client(id:int, connServers:set<int>)
 datatype DafnyState = DafnyState(clients:seq<Client>, servers:seq<Server>)
 
-// relation link(X:client, Y:server)
-// relation semaphore(X:server)
 predicate RelationLink(m: DafnyState, c: Client, s: Server)
 {
     && 0 <= s.id < |m.servers|
@@ -19,36 +15,34 @@ predicate RelationSemaphore(m: DafnyState, s: Server)
     && m.servers[s.id].semaphore
 }
 
-// after init {
-//     semaphore(W) := true;
-//     link(X,Y) := false
+// c1 should be not changing if it is != c2
+// predicate RelationLinkStable(m : DafnyState, m' : DafnyState, c1: Client, c2: Client, s: Server) {
+//     c1.id != c2.id ==> RelationLink(m, c1, s) == RelationLink(m', c1, s)  link_c1_s_next
 // }
-predicate Init(m: DafnyState) {
-    && forall s: Server :: s in m.servers ==> RelationSemaphore(m, s)
-    && forall s: Server, c: Client :: s in m.servers && c in m.clients ==> !RelationLink(m, c, s)
+
+predicate RelationDifferentClients(m: DafnyState, c1: Client, c2: Client){
+    c1.id != c2.id
 }
 
-// predicate ServerInit(s: Server, id: int) {
-//     s.semaphore == true && s.id == id
-// }
+predicate RelationDifferentServers(m: DafnyState, s1: Server, s2: Server){
+    s1.id != s2.id
+}
 
-// predicate ClientInit(c: Client, id: int) {
-//     |c.connServers| == 0  && c.id == id
-// }
+predicate RelationServerExists(m: DafnyState, s: Server){
+    s in m.servers
+}
 
-// predicate Connect(s: Server, s': Server, c: Client, c': Client) {
-//     && s.id == s'.id
-//     && c.id == c'.id
-//     && s.semaphore == true
-//     && s'.semaphore == false
-//     && s.id in c'.connServers
-// }
+predicate RelationClientExists(m: DafnyState, c: Client){
+    c in m.clients
+}
 
-// action connect(x:client,y:server) = {
-//   require semaphore(y);
-//   link(x,y) := true;
-//   semaphore(y) := false
-// }
+predicate Init(m: DafnyState) {
+    // && (forall s: Server :: s in m.servers ==> RelationSemaphore(m, s))
+    && (forall s: Server :: RelationServerExists(m, s) ==> RelationSemaphore(m, s))
+    // && (forall s: Server, c: Client :: s in m.servers && c in m.clients ==> !RelationLink(m, c, s))
+    && (forall s: Server, c: Client :: ((RelationServerExists(m, s) && RelationClientExists(m, c)) ==> !RelationLink(m, c, s)))
+}
+
 predicate ActionConnect(m: DafnyState, m': DafnyState) {
     exists c: Client, s: Server ::
 
@@ -57,27 +51,13 @@ predicate ActionConnect(m: DafnyState, m': DafnyState) {
         && !RelationSemaphore(m', s)
 
         // TODO: might need to ensure client/server is in m.clients/m.servers on left side of implication
-        && forall cf: Client, sf: Server :: (cf.id != c.id ==> RelationLink(m, cf, sf) == RelationLink(m', cf, sf))
+        // && forall cf: Client, sf: Server :: (cf.id != c.id ==> RelationLink(m, cf, sf) == RelationLink(m', cf, sf))
+        // && forall cf: Client, sf: Server :: RelationLinkStable(m, cf, c, sf)
+        && forall cf: Client, sf: Server :: (RelationDifferentClients(m, cf, c) ==> RelationLink(m, cf, sf) == RelationLink(m', cf, sf))
         
-        && forall sf: Server :: (sf.id != s.id ==> RelationSemaphore(m, sf) == RelationSemaphore(m', sf))
-
-
-        /*
-        && c in m.clients // client exists
-        && s in m.servers // server exists
-        && s.semaphore == true // server is unlocked to start
-        && Client(c.id, c.connServers + {s.id}) in m'.clients // client ends up locked on this server
-        && Server(s.id, false) in m'.servers // server ends up locked
-        && (m.servers - {s}) == (m'.servers - {Server(s.id, false)}) // no other changes
-        && (m.clients - {c}) == (m'.clients - {Client(c.id, c.connServers + {s.id})}) // no other changes
-        */
+        && forall sf: Server :: (RelationDifferentServers(m, sf, s) ==> RelationSemaphore(m, sf) == RelationSemaphore(m', sf))
 }
 
-// action disconnect(x:client,y:server) = {
-//   require link(x,y);
-//   link(x,y) := false;
-//   semaphore(y) := true
-// }
 predicate ActionDisconnect(m: DafnyState, m': DafnyState) {
     exists c: Client, s: Server ::
 
@@ -85,34 +65,23 @@ predicate ActionDisconnect(m: DafnyState, m': DafnyState) {
         && !RelationLink(m', c, s)
         && RelationSemaphore(m', s)
 
-        && forall cf: Client, sf: Server :: (cf.id != c.id ==> RelationLink(m, cf, sf) == RelationLink(m', cf, sf))
+        && forall cf: Client, sf: Server :: (RelationDifferentClients(m, cf, c) ==> RelationLink(m, cf, sf) == RelationLink(m', cf, sf))
         
-        && forall sf: Server :: (sf.id != s.id ==> RelationSemaphore(m, sf) == RelationSemaphore(m', sf))
+        && forall sf: Server :: (RelationDifferentServers(m, sf, s) ==> RelationSemaphore(m, sf) == RelationSemaphore(m', sf))
 
-   /* && c in m.clients // client exists
-    && s in m.servers // server exists
-    && s.id in c.connServers // client held server lock
-    && Client(c.id, c.connServers - {s.id}) in m'.clients // client ends up unlocked on this server
-    && Server(s.id, true) in m'.servers // server ends up unlocked
-    && (m.servers - {s}) == (m'.servers - {Server(s.id, true)}) // no other changes
-    && (m.clients - {c}) == (m'.clients - {Client(c.id, c.connServers - {s.id})}) // no other changes*/
 }
 
 predicate Next(m:DafnyState, m':DafnyState) {
-    //|| (exists c:Client, s:Server :: Connect(m, m', c, s))
-    //|| (exists c:Client, s:Server :: Disconnect(m, m', c, s))
     || ActionConnect(m, m')
     || ActionDisconnect(m, m')
 }
 
-// export connect
-// export disconnect
 
-// invariant [1000000] link(C1, S) & link(C2, S) -> C1 = C2
 lemma Invariant(m: DafnyState) 
     ensures forall c1: Client, c2:Client, s: Server :: 
-    (c1 in m.clients && c2 in m.clients && s in m.servers) ==> (RelationLink(m, c1, s) && RelationLink(m, c2, s) ==> c1.id == c2.id)
+    (RelationClientExists(m, c1) && RelationClientExists(m, c2) && RelationServerExists(m, s)) ==> (RelationLink(m, c1, s) && RelationLink(m, c2, s) ==> !RelationDifferentClients(m, c1, c2))
 {
     // somehow need to prove that safety property
 }
+
 
