Test/591tests/switch_state_ours.dfy
@@ -1,0 +1,38 @@
+//#instructor The switch is an example of a very simple state machine.
+//#instructor All its steps are non-parameterized.
+//#instructor This example is intended to show the basic of the boilerplate
+//#instructor of a TLA+ state machine embedded in Dafny.
+
+datatype SwitchState = On | Off
+
+datatype DafnyState = Whatever(switch:SwitchState)
+
+predicate RelationSwitchOn(v: DafnyState) {
+    v.switch == On
+}
+
+predicate Init(v:DafnyState) {
+    // v.switch == Off
+    !RelationSwitchOn(v)
+}
+
+predicate ActionActivate(v:DafnyState, v':DafnyState) {
+    // v'.switch == On
+    RelationSwitchOn(v')
+}
+
+predicate ActionDeactivate(v:DafnyState, v':DafnyState) {
+    // v'.switch == Off
+    !RelationSwitchOn(v')
+}
+
+predicate ActionToggle(v:DafnyState, v':DafnyState) {
+    // v'.switch == if v.switch.On? then Off else On
+    RelationSwitchOn(v') != RelationSwitchOn(v)
+}
+
+predicate Next(v:DafnyState, v':DafnyState) {
+    || ActionActivate(v, v')
+    || ActionDeactivate(v, v')
+    || ActionToggle(v, v')
+}
